

## Intermediate value theorem, numerical equation solving

Suppose we want to numerically solve the equation  $f(x) = 0$  for  $x \in [a, b]$ . A reasonable assumption to make is that  $f(a) < 0 < f(b)$ . The intermediate value theorem asserts that a solution *exists*, but it doesn't tell us how to find it. We can look at the proof of the IVT for a lead, but all that says is that the solution is

$$c = \sup \{x \in [a, b] : f(x) < 0\}$$

which we still can't compute. The following two problems outline a new proof of the intermediate value theorem that's more useful for numerical purposes.

The following problem is needed in the proof, it's called the *nested interval theorem*.

1. (a) Suppose that  $A$  and  $B$  are two non-empty sets of numbers such that  $x \leq y$  for all  $x \in A$  and  $y \in B$ . Show that  $\sup A \leq \inf B$ .  
(b) Consider a sequence of closed intervals  $I_1 = [a_1, b_1], I_2 = [a_2, b_2], \dots$ . Suppose that  $a_n \leq a_{n+1}$  and  $b_n \geq b_{n+1}$  for all  $n$ . Prove that there is a point  $x$  which is in every  $I_n$ .

*Solution.* Lets do part (a) first since we need it for part (b). Let  $\alpha = \sup A$  and  $\beta = \sup B$ . Notice that every element of  $B$  is an upper bound of  $A$ . Therefore  $\alpha \leq b$  for all  $b \in B$ , and with similar reasoning we can conclude that  $\beta \geq a$  for all  $a \in A$ . This means that  $\alpha$  is a lower bound for  $B$ , and  $\beta$  is a lower bound for  $A$ . Thus  $\alpha \leq \beta$  since  $\alpha$  is the *least* upper bound and  $\beta$  is the *greatest* lower bound.

For the second part, we need to show that  $A = \{a_n : n \in \mathbb{N}\}$  and  $B = \{b_n : n \in \mathbb{N}\}$  satisfy the hypotheses of part (a). That is, we have to demonstrate that  $a_n \leq b_m$  for any naturals  $n$  and  $m$ . This holds because

$$a_n \leq a_{n+m} \leq b_{n+m} \leq b_m$$

and these inequalities hold because the intervals are nested within each other.

Therefore  $\sup A \leq \inf B$ , meaning that the interval  $[\sup A, \inf B]$  is non-empty, and is a subset of  $I_n$  for all  $n$ . This is what we wanted to show.  $\square$

2. (a) Suppose  $f$  is continuous  $[a, b]$  and  $f(a) < 0 < f(b)$ . Consider the midpoint  $m_1 = (a + b)/2$ . Either,
  - $f(m_1) = 0$ ,
  - $f(m_1) > 0$ , in which case  $f(a)$  and  $f(m_1)$  have different signs
  - $f(m_1) < 0$ , in which case  $f(m_1)$  and  $f(b)$  have different signs.Use this to find an interval  $I_1$  such that  $f$  has different signs on its endpoints. Repeat this process more times to find a nested sequence of intervals  $I_1 \supset I_2 \supset \dots$ .  
(b) Use the nested interval theorem to find a solution to the equation  $f(x) = 0$ .

*Solution.* We will specify the intervals  $I_n$  by their endpoints  $[a_n, b_n]$ , and let  $m_n = (a_n + b_n)/2$  denote the midpoint of the  $n$ th interval. Let  $I_0 = [a, b]$ ,

and define  $I_{n+1}$  iteratively using  $I_n$  as follows

$$I_{n+1} = \begin{cases} \{m_n\} & f(m_n) = 0 \\ [a_n, m_n] & f(m_n)f(a_n) < 0 \\ [m_n, b_n] & f(m_n)f(b_n) < 0 \end{cases}$$

Notice that, in all cases,  $I_{n+1} \subset I_n$ . As such, the sets so constructed will satisfy  $I_1 \supset I_2 \supset \dots$ . The previous problem tells us that there is a point  $c$  that lies in all of these intervals.

Suppose for the sake of contradiction that  $f(c) > 0$ . This means that  $f$  is positive on some interval  $J = (c - \delta, c + \delta)$  about  $c$ . Note that this interval has length  $2\delta$ . However,  $I_n$  has length  $(b - a)/2^n$  so if we pick  $n$  big enough such that  $(b - a)/2^n < \delta$ , then  $I_n = [a_n, b_n] \subset J$ . Because of the way we constructed the  $I_n$ 's, we know that  $f$  is negative at some point of  $I_n$ , contradicting that  $f$  is positive on  $J$ . Therefore  $f(c) = 0$ .  $\square$

Some of you may have noticed that this is similar to the binary search algorithm for a list. The implementation on a computer is going to be similar.

**3 (Bonus, numerical analysis).** Implement an algorithm based on the proof above that solves equations involving continuous functions. Use this algorithm to approximate the root of  $x^3 - 3x + 1$ . Your algorithm must allow the user to specify the tolerance value  $\varepsilon$ , and the output  $x$  of your algorithm must satisfy  $|f(x)| < \varepsilon$ .

If you are working with python, you can try and extend

```
def solve(f, a, b, tolerance):
    pass
```

## The derivative

**4.** Find  $f'(a)$  where (a)  $f(x) = x^n$  for  $n \geq 2$ , (b)  $f(x) = 1/x$  and (c)  $f(x) = \sin x$ .

*Solution.*

$$\begin{aligned} f'(a) &= \lim_{h \rightarrow 0} \frac{(a+h)^n - a^n}{h} \\ &= \lim_{h \rightarrow 0} \frac{\sum_{k=0}^n \binom{n}{k} a^{n-k} h^k - a^n}{h} \\ &= \lim_{h \rightarrow 0} \frac{na^{n-1}h + \binom{n}{2}a^{n-2}h^2 + \dots}{h} \\ &= \lim_{h \rightarrow 0} \left( na^{n-1} + \binom{n}{2}a^{n-2}h + \dots \right) \\ &= na^{n-1} \end{aligned}$$

$$\begin{aligned}
f'(a) &= \lim_{h \rightarrow 0} \frac{\frac{1}{a+h} - \frac{1}{a}}{h} \\
&= \lim_{h \rightarrow 0} \frac{a - (a+h)}{a(a+h)h} \\
&= \lim_{h \rightarrow 0} \frac{-1}{a(a+h)} \\
&= -\frac{1}{a^2}
\end{aligned}$$

$$\begin{aligned}
f'(a) &= \lim_{h \rightarrow 0} \frac{\sin(a+h) - \sin a}{h} \\
&= \lim_{h \rightarrow 0} \frac{\sin a(\cos h - 1) + \cos a \sin h}{h} \\
&= \sin a \cdot \lim_{h \rightarrow 0} \frac{\cos h - 1}{h} + \cos a \cdot \lim_{h \rightarrow 0} \frac{\sin h}{h} \\
&= \cos a
\end{aligned}$$

□

**5.** What are the slopes of the tangents to the curves  $f(x) = 1/x$  and  $g(x) = x^2$  at the point of their intersection? Find the angle between these tangents.

*Solution.* Where do these curves intersect?

$$x^2 = \frac{1}{x} \implies x^3 = 1 \implies x = 1$$

Using the results from a previous question we conclude that  $f'(1) = 2$  and  $g'(1) = -1$ .

The angle of inclination of the first line is  $\theta = \arctan 2$ , and the second line is  $\phi = \arctan(-1)$ . Therefore the angle between the two lines is  $\arctan(2) - \arctan(-1) = \arctan(2) + \arctan(1)$ . □

**6.** Find  $f'(0)$ ,  $f'(1)$ , and  $f'(2)$  where  $f(x) = x(x-1)^2(x-2)^3$ .

*Solution.*

$$\begin{aligned}
f'(0) &= \lim_{h \rightarrow 0} \frac{f(h) - f(0)}{h} \\
&= \lim_{h \rightarrow 0} \frac{h(h-1)^2(h-2)^3 - 0}{h} \\
&= \lim_{h \rightarrow 0} (h-1)^2(h-2)^3 \\
&= (0-1)^2(0-2)^3 \\
&= -8
\end{aligned}$$

$$\begin{aligned}
f'(1) &= \lim_{h \rightarrow 0} \frac{f(1+h) - f(1)}{h} \\
&= \lim_{h \rightarrow 0} \frac{(1+h)h^2(h-1)^3 - 0}{h} \\
&= \lim_{h \rightarrow 0} h(1+h)(h-1)^3 \\
&= 0
\end{aligned}$$

$$\begin{aligned}
f'(2) &= \lim_{h \rightarrow 0} \frac{f(2+h) - f(2)}{h} \\
&= \lim_{h \rightarrow 0} \frac{(2+h)(1+h)^2h^3 - 0}{h} \\
&= \lim_{h \rightarrow 0} (2+h)(1+h)^2h^2 \\
&= 0
\end{aligned}$$

□